Dafny/14_insertionSort.01.dfy
@@ -1,7 +1,88 @@
 // Insertion sort
 
-include "displace.dfy"
-include "find.dfy"
+predicate sorted(s: seq<int>)
+{
+  forall i,j :: 0 <= i < j < |s| ==> s[i] <= s[j]
+}
+
+method findIns(arr: array<int>, val: int, len: nat) returns (r: nat)
+requires arr != null
+requires len < arr.Length
+// arr is an ordered array
+requires sorted(arr[..len])
+// return value should not exceed len
+ensures r <= len
+// index of place of insertion is returned
+ensures forall k: nat :: k < r ==> arr[k] < val
+ensures sorted( arr[..r] + [val] + arr[r..len] )
+{
+  r := 0;
+  
+  while r < len
+    invariant r <= len
+    decreases len - r
+    invariant forall k: nat :: k < r ==> arr[k] < val
+    invariant arr == old(arr)
+    {
+      if arr[r] >= val
+      { return; }
+      r := r + 1;
+    }
+}
+
+predicate rotated(arr1:seq<int>, arr2:seq<int>) 
+  requires |arr1| == |arr2|
+{
+  (forall i :: 1 <= i < |arr1| ==> arr2[i] == arr1[i - 1]) &&
+      ( |arr1| > 0 ==> arr2[0] == arr1[ |arr1| - 1 ] )
+}
+
+method displace(arr: array<int>, start: nat, len: nat)
+    returns (r: array<int>)
+  requires arr != null
+  requires len > 0
+  requires start + len <= arr.Length
+  ensures r != null && r.Length == arr.Length
+  ensures arr[..start] == r[..start]
+  ensures arr[(start + len)..] == r[(start + len)..]
+  ensures rotated(arr[start .. start+len], r[start .. start+len])
+{
+  var i: nat := 0;
+  r := new int[arr.Length];
+  while i < start
+    invariant i <= start
+    invariant forall k: nat :: k < i ==> r[k] == arr[k]
+    {
+      r[i] := arr[i];
+      i := i + 1;
+    }
+    assert arr[..start] == r[..start];
+  r[start] := arr[start+len-1];
+  assert r[start] == arr[start+len-1];
+  
+  i := start+1;
+  while i < start+len
+    invariant start < i <= start+len
+    invariant arr[..start] == r[..start]
+    invariant r[start] == arr[start+len-1]
+    invariant forall k: nat :: start < k < i ==> r[k] == arr[k-1]
+    {
+      r[i] := arr[i-1];
+      i := i + 1;
+    }
+    assert rotated(arr[start .. start+len], r[start .. start+len]);
+  
+  i := start+len;
+  while i < arr.Length
+    invariant start+len <= i <= arr.Length
+    invariant arr[..start] == r[..start]
+    invariant rotated(arr[start .. start+len], r[start .. start+len])
+    invariant forall k: nat :: start+len <= k < i ==> r[k] == arr[k]
+    {
+      r[i] := arr[i];
+      i := i + 1;
+    }
+}
 
 method insertSort(arr: array<int>) returns (r: array<int>)
   requires arr != null
@@ -12,9 +93,11 @@ method insertSort(arr: array<int>) returns (r: array<int>)
     var i: nat := 0;
     var pos: nat := 0;
     r := new int[arr.Length];
+    assert r != null;
     
     while (i < r.Length)
       invariant i <= r.Length
+      invariant arr.Length == r.Length
       invariant forall k: nat :: k < i ==> r[k] == arr[k]
     {
         r[i] := arr[i];
@@ -23,9 +106,8 @@ method insertSort(arr: array<int>) returns (r: array<int>)
     assert r[..] == arr[..];
     i := 0;
     while (i < r.Length)
-      //...
-      //invariant r != null
-      //decreases r.Length - i
+      invariant r != null
+      decreases r.Length - i
       invariant i <= r.Length
       invariant arr.Length == r.Length
       invariant sorted( r[..i] )
@@ -34,4 +116,5 @@ method insertSort(arr: array<int>) returns (r: array<int>)
         i := i + 1;
         r := displace(r, pos, i - pos);
     }
+    assert sorted( r[..i] );
 }
