Whiley/01_palindrome.01.whiley
@@ -9,7 +9,7 @@ function isPalindrome(int[] chars) -> (bool r)
   
   while i < j
     where i + j == |chars| && i >= 0
-    where all { k in 0..i | chars[k] == chars[|chars| - (k+1)] }
+    where all { k in 0..i | chars[k] == chars[|chars| - (k + 1)] }
   :
     j = j - 1
     if chars[i] != chars[j]
